Clean up the Coq formalization.

MicroProver.v
@@ -19,6 +19,7 @@ Inductive form : Type :=
 | Falsity
 | Imp (p : form) (q : form).
 
+(* Before we can form MSets of formulas, we need to show that they are a decidable type *)
 Module Form_As_DT <: DecidableType.
   Definition t := form.
   Definition eq := @eq form.
@@ -31,11 +32,13 @@ Module Form_As_DT <: DecidableType.
   Proof using Type Type. intros. unfold eq. decide equality. decide equality. Qed.
 End Form_As_DT.
 
+(* Now we can obtain MSets of formulas and a number of theorems about them *)
 Module Import S := Make Form_As_DT.
 Module Import MSetDec := MSetDecide.WDecide S.
 Module Import MSetFacts := MSetFacts.WFacts S.
 Module Import MSetProps := MSetProperties.WProperties S.
 Module Import MSetEqProps := MSetEqProperties.WEqProperties S.
+Infix "[+]" := add (at level 81, right associativity).
 
 (* Semantics is a predicate over an interpretation i determining
    whether the formula is true for the given interpretation. *)
@@ -46,9 +49,11 @@ Fixpoint semantics (i : nat -> bool) (f : form) : Prop :=
   | Imp p q => semantics i p -> semantics i q
   end.
 
+(* The semantics function is decidable, which we will need to
+   perform proofs by case analysis on the semantics *)
 Lemma semantics_dec : forall i f, decidable (semantics i f).
 Proof using Type.
-  intros. unfold decidable. induction f.
+  intros. unfold decidable. induction f as [ | | IHf1 IHf2 ].
   - simpl. destruct (i n); auto.
   - simpl. auto.
   - simpl. destruct IHf1; destruct IHf2; intuition.
@@ -61,16 +66,20 @@ Definition sc (x y : t) (i : nat -> bool) : Prop :=
   For_all (semantics i) x -> Exists (semantics i) y.
 
 (* We define a sequent calculus as an inductive predicate. *)
-Inductive SC : t -> t -> Prop :=
-| Fls_L X Y : SC (add Falsity X) Y
-| Imp_L p q X Y (H1: SC X (add p Y)) (H2: SC (add q X) Y)
-  : SC (add (Imp p q) X) Y
-| Imp_R p q X Y (H: SC (add p X) (add q Y)) : SC X (add (Imp p q) Y)
-| Set_L X X' Y (H1: SC X Y) (H2: eq X' X) : SC X' Y
-| Set_R Y X Y' (H1: SC X Y) (H2: eq Y' Y) : SC X Y'
-| Basic p X Y : SC (add p X) (add p Y).
 
-(* This tactic proves equality of two sets, which is useful for the Set_L and Set_R rules. *)
+Reserved Infix ">>" (at level 90, no associativity).
+Inductive SC : t -> t -> Prop :=
+| Fls_L X Y : Falsity [+] X >> Y
+| Imp_L p q X Y (H1: X >> p [+] Y) (H2: q [+] X >> Y)
+  : Imp p q [+] X >> Y
+| Imp_R p q X Y (H: p [+] X >> q [+] Y) : X >> (Imp p q [+] Y)
+| Set_L X X' Y (H1: X >> Y) (H2: eq X' X) : X' >> Y
+| Set_R Y X Y' (H1: X >> Y) (H2: eq Y' Y) : X >> Y'
+| Basic p X Y : (p [+] X) >> (p [+] Y)
+where "X >> Y" := (SC X Y).
+
+(* This tactic proves equality of two concrete sets, which is useful
+   for the Set_L and Set_R rules in the examples below. *)
 Ltac prove_set_equality := simpl; unfold eq; unfold Equal; intros; split;
                        let a := fresh "H" in
                        intros a; repeat rewrite add_spec in a;
@@ -80,25 +89,25 @@ Ltac prove_set_equality := simpl; unfold eq; unfold Equal; intros; split;
                        subst; repeat rewrite add_spec; intuition.
 
 (* We can use the sequent calculus as a proof system to prove various formulas. *)
-Example SC_ex1 : SC empty (of_list [Imp (Pro 0) (Pro 0)]).
+Example SC_ex1 : empty >> (of_list [Imp (Pro 0) (Pro 0)]).
 Proof using Type. apply Imp_R. apply Basic. Qed.
 
-Example SC_ex2 : SC empty (of_list [Imp (Pro 0) (Imp (Imp (Pro 0) (Pro 1)) (Pro 1))]).
+Example SC_ex2 : empty >> (of_list [Imp (Pro 0) (Imp (Imp (Pro 0) (Pro 1)) (Pro 1))]).
 Proof using Type. repeat apply Imp_R. apply Imp_L; apply Basic. Qed.
 
-Example SC_ex3 : SC empty (of_list [Imp (Pro 0) (Imp (Pro 1) (Imp (Pro 1) (Pro 0)))]).
+Example SC_ex3 : empty >> (of_list [Imp (Pro 0) (Imp (Pro 1) (Imp (Pro 1) (Pro 0)))]).
 Proof using Type. repeat apply Imp_R. apply (Set_L (of_list [Pro 0; Pro 1; Pro 1])).
        - apply Basic.
        - prove_set_equality.
 Qed.
 
-Example SC_ex4 : SC empty (of_list [Imp (Pro 0) (Imp (Imp (Pro 0) Falsity) Falsity)]).
+Example SC_ex4 : empty >> (of_list [Imp (Pro 0) (Imp (Imp (Pro 0) Falsity) Falsity)]).
 Proof using Type. repeat apply Imp_R. apply Imp_L.
        - apply Basic.
        - apply Fls_L.
 Qed.
 
-Example SC_ex5 : SC empty (of_list [Imp (Imp (Imp (Pro 0) (Falsity)) (Falsity)) (Pro 0)]).
+Example SC_ex5 : empty >> (of_list [Imp (Imp (Imp (Pro 0) (Falsity)) (Falsity)) (Pro 0)]).
 Proof using Type. repeat apply Imp_R. apply Imp_L.
        - apply Imp_R. apply (Set_R (of_list [Pro 0; Falsity])).
          + apply Basic.
@@ -108,61 +117,61 @@ Qed.
 
 Example sc_ex1 : forall i, sc empty (of_list [Imp (Imp (Imp (Pro 0) (Falsity)) (Falsity)) (Pro 0)]) i.
 Proof using Type.
-  unfold sc. intros. destruct (i 0) eqn:EP.
+  unfold sc. intros i Hempty. destruct (i 0) eqn:EP.
   - unfold Exists. exists (Imp (Imp (Imp (Pro 0) Falsity) Falsity) (Pro 0)). split.
     + apply add_spec. intuition.
     + simpl. intuition.
   - unfold Exists. exists (Imp (Imp (Imp (Pro 0) Falsity) Falsity) (Pro 0)). split.
     + apply add_spec. intuition.
-    + simpl. intros. exfalso. apply H0. intros. rewrite EP in H1. inversion H1.
+    + simpl. intros. exfalso. apply H. intros H'. rewrite EP in H'. inversion H'.
 Qed.
 
 (* The proof system above is sound in the sense that if there is a proof
    in it, the sc predicate is true. *)
 
-Lemma sound_imp_l : forall p q l r i, sc l (add p r) i -> sc (add q l) r i -> sc (add (Imp p q) l) r i.
+Lemma sound_imp_l : forall p q l r i, sc l (p [+] r) i -> sc (q [+] l) r i -> sc ((Imp p q) [+] l) r i.
 Proof.
-  unfold sc. intros.
-  destruct (semantics_dec i (Imp p q)).
-  - unfold For_all in H1.
-    assert (forall x, In x l -> semantics i x).
-    { intros. apply H1. apply add_spec. intuition. }
-    specialize (H H3). unfold Exists in H. destruct H as [x [HxIn Hx]].
+  unfold sc. intros p q l r i Hp Hq Hpq.
+  destruct (semantics_dec i (Imp p q)) as [H | H].
+  - unfold For_all in Hpq.
+    assert (Hxl: forall x, In x l -> semantics i x).
+    { intros. apply Hpq. apply add_spec. intuition. }
+    specialize (Hp Hxl). unfold Exists in Hp. destruct Hp as [x [HxIn Hx]].
     apply add_spec in HxIn. destruct HxIn.
-    + subst. apply H0. unfold For_all. intros. apply add_spec in H.
-      destruct H.
-      * subst. simpl in H2. intuition.
+    + subst. apply Hq. unfold For_all. intros x Hx'. apply add_spec in Hx'.
+      destruct Hx'.
+      * subst. simpl in Hpq. intuition.
       * intuition.
     + unfold Exists. exists x. intuition.
-  - assert (semantics i (Imp p q)).
-    { unfold For_all in H1. apply H1. apply add_spec. intuition. }
+  - assert (Himp: semantics i (Imp p q)).
+    { unfold For_all in Hq. apply Hpq. apply add_spec. intuition. }
     intuition.
 Qed.
 
 Lemma semantics_imp : forall p q i, ~ semantics i (Imp p q) -> semantics i p /\ ~ semantics i q.
 Proof.
-  intros. split.
+  intros p q i H. split.
   - destruct (semantics_dec i p).
     + assumption.
-    + exfalso. apply H. simpl. intros. contradiction.
+    + exfalso. apply H. simpl. intuition.
   - destruct (semantics_dec i q).
-    + exfalso. apply H. simpl. intros. assumption.
+    + exfalso. apply H. simpl. intuition.
     + assumption.
 Qed.
 
-Lemma sound_imp_r : forall p q l r i, sc (add p l) (add q r) i -> sc l (add (Imp p q) r) i.
+Lemma sound_imp_r : forall p q l r i, sc (p [+] l) (q [+] r) i -> sc l (Imp p q [+] r) i.
 Proof.
-  unfold sc. intros.
-  destruct (semantics_dec i (Imp p q)).
+  unfold sc. intros p q l r i Hsc Hl.
+  destruct (semantics_dec i (Imp p q)) as [ | H].
   - unfold Exists. exists (Imp p q). split.
     + apply add_spec. intuition.
     + intuition.
-  - apply semantics_imp in H1. destruct H1 as [Hp Hnq].
+  - apply semantics_imp in H. destruct H as [Hp Hnq].
     assert (Hpl: For_all (semantics i) (add p l)).
-    { unfold For_all. intros. apply add_spec in H1. destruct H1.
+    { unfold For_all. intros. apply add_spec in H. destruct H.
       - subst. assumption.
       - intuition. }
-    specialize (H Hpl). unfold Exists in H. destruct H as [x [Hxq Hx]].
+    specialize (Hsc Hpl). unfold Exists in Hsc. destruct Hsc as [x [Hxq Hx]].
     apply add_spec in Hxq. destruct Hxq.
     + subst. intuition.
     + unfold Exists. exists x. split.
@@ -170,42 +179,38 @@ Proof.
       * intuition.
 Qed.
 
-Theorem sound_sc : forall X Y i,  SC X Y -> sc X Y i.
+Theorem sound_sc : forall X Y i, X >> Y -> sc X Y i.
 Proof.
-  intros X Y i HSC. induction HSC.
+  intros X Y i HSC. induction HSC as [ | | | X X' Y HSC IH Heq | Y X Y' HSC IH Heq | ].
   - unfold sc. intros H. unfold For_all in H.
     specialize (H Falsity). simpl in H. exfalso.
     rewrite add_spec in H. intuition.
   - apply sound_imp_l; assumption.
   - apply sound_imp_r; assumption.
-  - unfold sc. unfold eq in H2. unfold Equal in H2. unfold For_all. intros.
-    unfold For_all in IHHSC. apply IHHSC. unfold For_all. intros. apply H.
-    apply H2. assumption.
-  - unfold sc. unfold eq in H2. unfold Equal in H2. unfold Exists. intros.
-    unfold Exists in IHHSC. specialize (IHHSC H).
-    destruct IHHSC. exists x. rewrite H2. assumption.
+  - unfold sc. unfold eq in Heq. unfold Equal in Heq. unfold For_all. intros.
+    unfold For_all in IH. apply IH. unfold For_all. intros. intuition.
+  - unfold sc. unfold eq in Heq. unfold Equal in Heq. unfold Exists. intros.
+    unfold Exists in IH. specialize (IH H). destruct IH. exists x. rewrite Heq. assumption.
   - unfold sc. intros H. unfold Exists. unfold For_all in H. exists p. split.
     + apply add_spec. intuition.
     + apply H. apply add_spec. intuition.
 Qed.
 
 (* Specifically, a proof of a single formula means that the formula is semantically valid *)
-
-Corollary sound : forall i p, SC empty (singleton p) -> semantics i p.
+Corollary sound : forall i p, empty >> singleton p -> semantics i p.
 Proof.
   intros i p H. apply (sound_sc _ _ i) in H. unfold sc in H.
   destruct H.
   - unfold For_all. intros. apply empty_spec in H. contradiction.
-
-  - intuition. apply singleton_spec in H0. subst. assumption.
+  - destruct H as [Hin Hx]. apply singleton_spec in Hin. subst. assumption.
 Qed.
 
-(* Now we want to define a prover, but first we need some executable helper functions  *)
+(* Now we want to define a prover, but first we need some executable helper functions *)
 
 Fixpoint member (x : nat) (xs : list nat) : bool :=
   match xs with
   | [] => false
-  | y :: ys => if Nat.eqb x y then true else member x ys
+  | y :: ys => if x =? y then true else member x ys
   end.
 
 Fixpoint common (a b : list nat) : bool :=
@@ -214,7 +219,8 @@ Fixpoint common (a b : list nat) : bool :=
   | m :: ms => if member m a then true else common a ms
   end.
 
-(* We define a notion of size for formulas and lists of formulas *)
+(* We also need a notion of size for formulas and lists of formulas
+   for our termination proofs *)
 Fixpoint form_size (f : form) : nat :=
   match f with
   | Pro _ => 1
@@ -243,17 +249,19 @@ Equations? mp (a b : list nat) (c d: list form) : bool by wf (forms_size c + for
   mp a b [] [] => common a b.
 Proof. all: try apply lt_n_S; lia. Qed.
 
+(* We can specialize this function to a prover for a single formula *)
 Definition prover (p : form) : bool := mp [] [] [] [p].
 
-(* We now want to prove that the prover mp is sound and complete with regards
+(* We now want to prove that the prover is sound and complete with regards
    to the semantics. *)
 
-(* But first, we take a detour to specify a prover that returns counterexamples, since
-   we will need more information than just a boolean value to actually prove
+(* To do this, we first take a detour to specify a prover that returns counterexamples,
+   since we will need more information than just a boolean value to actually prove
    completeness. *)
 
-(* We define a prover that returns the information necessary to build counterexamples *)
-Equations? mu (a b : list nat) (c d : list form) : list (list nat) by wf (forms_size c + forms_size d) lt :=
+(* We thus define a prover that returns the information necessary to build counterexamples *)
+Equations? mu (a b : list nat) (c d : list form) : list (list nat)
+  by wf (forms_size c + forms_size d) lt :=
   mu a b (Pro n :: c) [] => mu (n :: a) b c [];
   mu a b (Pro m :: c) (Pro n :: d) => mu a (n :: b) (Pro m :: c) d;
   mu a b c (Pro n :: d) => mu a (n :: b) c d;
@@ -265,23 +273,24 @@ Equations? mu (a b : list nat) (c d : list form) : list (list nat) by wf (forms_
   mu a b [] [] => if common a b then [] else [a].
 Proof. all: try apply lt_n_S; lia. Qed.       
 
-Lemma set_in_add : forall x s, In x s -> exists s', Equal s (add x s').
+(* Before we can prove soundness and completeness, we need to prove a
+   few properties about sets and our proof system *)
+Lemma set_in_add : forall x s, In x s -> exists s', Equal s (x [+] s').
 Proof.
-  intros. exists (remove x s). unfold Equal. intros. split.
-  - intros. apply add_spec. rewrite remove_spec.
-    destruct (Form_As_DT.eq_dec a x).
+  intros x s H. exists (remove x s). unfold Equal. intros a. split.
+  - intros H'. apply add_spec. rewrite remove_spec.
+    destruct (Form_As_DT.eq_dec a x) as [e | n].
     + unfold Form_As_DT.eq in e. intuition.
     + unfold Form_As_DT.eq in n. intuition.
-  - rewrite add_spec. rewrite remove_spec. intros.
-    destruct H0.
+  - rewrite add_spec. rewrite remove_spec. intros H'. destruct H'.
     + subst. assumption.
     + intuition.
 Qed.
 
-Lemma shared_proven : forall x l r, In x l -> In x r -> SC l r.
+Lemma shared_proven : forall x l r, In x l -> In x r -> l >> r.
 Proof.
-  intros. apply set_in_add in H. apply set_in_add in H0.
-  destruct H as [l' Hl']. destruct H0 as [r' Hr'].
+  intros x l r Hl Hr. apply set_in_add in Hl. apply set_in_add in Hr.
+  destruct Hl as [l' Hl']. destruct Hr as [r' Hr'].
   apply (Set_L (add x l')); try assumption.
   apply (Set_R (add x r')); try assumption.
   apply Basic.
@@ -289,35 +298,35 @@ Qed.
 
 Lemma member_In : forall x xs, member x xs = true <-> List.In x xs.
 Proof.
-  split; intros.
-  - induction xs.
+  intros x xs. split; intros H.
+  - induction xs as [ | x' xs' IH].
     + inversion H.
-    + simpl in *. destruct (x =? a) eqn: Hxa.
-      * apply Nat.eqb_eq in Hxa. intuition.
+    + simpl in *. destruct (x =? x') eqn: Heq.
+      * apply Nat.eqb_eq in Heq. intuition.
       * intuition.
-  - induction xs.
+  - induction xs as [| x' xs' IH].
     + inversion H.
-    + inversion H.
+    + inversion H as [Heq | Hin].
       * subst. simpl. rewrite Nat.eqb_refl. reflexivity.
-      * specialize (IHxs H0). simpl. rewrite IHxs. destruct (x =? a); intuition.
+      * specialize (IH Hin). simpl. rewrite IH. destruct (x =? x'); intuition.
 Qed.
 
 Lemma common_spec : forall a b, common a b = true -> exists x, List.In x a /\ List.In x b.
 Proof.
-  intros. induction b.
+  intros a b H. induction b as [ | b' bs IH].
   - inversion H.
-  - destruct a.
-    + simpl in *. specialize (IHb H). destruct IHb as [_ [contra _]]. contradiction.
-    + destruct (a0 =? n) eqn:Hn.
-      * exists n. apply Nat.eqb_eq in Hn. subst. intuition.
-      * simpl in H. rewrite Hn in H. destruct (member a0 a) eqn: Ha.
-        -- exists a0. apply member_In in Ha. split; intuition.
-        -- specialize (IHb H). destruct IHb as [x [Hxa Hxb]]. exists x. intuition.
+  - destruct a as [ | a' as' ].
+    + simpl in *. specialize (IH H). destruct IH as [_ [contra _]]. contradiction.
+    + destruct (b' =? a') eqn:Hab.
+      * exists a'. apply Nat.eqb_eq in Hab. subst. intuition.
+      * simpl in H. rewrite Hab in H. destruct (member b' as') eqn: Hmem.
+        -- exists b'. apply member_In in Hmem. split; intuition.
+        -- specialize (IH H). destruct IH as [x []]. exists x. intuition.
 Qed.
 
 Lemma In_set : forall x b, List.In x b -> In x (of_list b).
 Proof.
-  intros. induction b.
+  intros x b H. induction b.
   - inversion H.
   - simpl. apply add_spec. destruct H; intuition.
 Qed.
@@ -329,30 +338,30 @@ Qed.
 
 Lemma of_list_comm : forall a b n, Equal (of_list (a ++ n :: b)) (of_list (n :: a ++ b)).
 Proof.
-  intros. induction a.
+  intros a b n. induction a as [| a' as' IH].
   - fsetdec.
   - split.
-    + intros. simpl in *. rewrite add_add. rewrite <- IHa. assumption.
-    + intros. simpl in *. rewrite add_add in H. rewrite IHa. assumption.
+    + intros. simpl in *. rewrite add_add. rewrite <- IH. assumption.
+    + intros H. simpl in *. rewrite add_add in H. rewrite IH. assumption.
 Qed.
 
-Lemma set_add_comm : forall x y A, eq (add x (add y A)) (add y (add x A)).
+Lemma set_add_comm : forall x y A, eq (x [+] y [+] A) (y [+] x [+] A).
   intros. unfold eq. unfold Equal. split.
-  - intros. apply add_spec in H. destruct H.
+  - intros H. apply add_spec in H. destruct H as [ | H].
     + apply add_spec. right. apply add_spec. intuition.
     + apply add_spec in H. destruct H.
       * apply add_spec. intuition.
       * apply add_spec. right. apply add_spec. intuition.
-  - intros. apply add_spec in H. destruct H.
+  - intros H. apply add_spec in H. destruct H as [ | H].
     + apply add_spec. right. apply add_spec. intuition.
     + apply add_spec in H. destruct H.
       * apply add_spec. intuition.
       * apply add_spec. right. apply add_spec. intuition.
 Qed.
 
-Lemma weaken : forall l r f, SC l r -> SC l (add f r).
+Lemma weaken : forall l r f, l >> r -> l >> f [+] r.
 Proof.
-  intros. induction H.
+  intros l r f H. induction H as [ | p q X Y | p q X Y | X X' Y | Y X Y' H Hf Heq | p X Y ].
   - apply Fls_L.
   - apply Imp_L.
     + apply (Set_R (add f (add p Y))); try assumption; apply set_add_comm.
@@ -361,72 +370,65 @@ Proof.
     apply Imp_R. apply (Set_R (add f (add q Y))); try assumption; apply set_add_comm.
   - apply (Set_L X); try assumption.
   - apply (Set_R (add f Y)); try assumption. unfold eq. unfold Equal. intros. split.
-    + intros. apply add_spec in H0. destruct H0.
+    + intros H'. apply add_spec in H'. destruct H'.
       * subst. apply add_spec. intuition.
-      * apply add_spec. right. unfold eq in H2. unfold Equal in H2. apply H2. assumption.
-    + intros. apply add_spec in H0. destruct H0.
+      * apply add_spec. right. unfold eq in Heq. unfold Equal in Heq. apply Heq. assumption.
+    + intros H'. apply add_spec in H'. destruct H'.
       * subst. apply add_spec. intuition.
-      * apply add_spec. right. unfold eq in H2. unfold Equal in H2. apply H2. assumption.
+      * apply add_spec. right. unfold eq in Heq. unfold Equal in Heq. apply Heq. assumption.
   - apply (Set_R (add p (add f Y))); try apply set_add_comm. apply Basic.
 Qed.
 
-
+(* We are now ready to prove the soundness of our counterexample-producing prover *)
 Lemma proven : forall a b c d, mu a b c d = [] -> SC (of_list (c ++ map Pro a)) (of_list (d ++ map Pro b)).
 Proof.
-  intros. funelim (mu a b c d).
-  - simpl. simp mu in H.
+  intros a b c d Hmu. funelim (mu a b c d).
+  - simpl. simp mu in Hmu.
     assert (Hc: common a b = true).
     { destruct (common a b); congruence. }
     apply common_spec in Hc. destruct Hc as [x [Hxa Hxb]].
     apply (in_set_map Pro) in Hxa. apply (in_set_map Pro) in Hxb.
     apply (shared_proven (Pro x)); assumption.
-  - simpl. simp mu in H0. specialize (H a (n :: b) [] d). intuition.
-    apply (Set_R (of_list (d ++ Pro n :: map Pro b))).
-    + assumption.
+  - simpl. simp mu in Hmu. apply (Set_R (of_list (d ++ Pro n :: map Pro b))).
+    + apply (H a (n :: b) [] d); intuition.
     + rewrite of_list_comm. simpl. unfold eq. fsetdec.
-  - simpl in *. simp mu in H0. specialize (H a b [] d). intuition.
-    apply weaken. assumption.
-  - simpl in *. simp mu in H0. specialize (H a b [p] (q :: d)). intuition.
-    apply Imp_R. intuition.
-  - simpl in *. simp mu in H0. specialize (H (n :: a) b c []). intuition.
-    apply (Set_L (of_list (c ++ Pro n :: map Pro a))).
-    + assumption.
+  - simpl in *. simp mu in Hmu. apply weaken. apply (H a b [] d); intuition.
+  - simpl in *. simp mu in Hmu. apply Imp_R. apply (H a b [p] (q :: d)); intuition.
+  - simpl in *. simp mu in Hmu. apply (Set_L (of_list (c ++ Pro n :: map Pro a))).
+    + apply (H (n :: a) b c []); intuition.
     + rewrite of_list_comm. simpl. unfold eq. fsetdec.
-  - simpl in *. simp mu in H0. specialize (H a (n :: b) (Pro m :: c) d). intuition.
-    apply (Set_R (of_list (d ++ map Pro (n :: b)))).
-    + assumption.
+  - simpl in *. simp mu in Hmu. apply (Set_R (of_list (d ++ map Pro (n :: b)))).
+    + apply (H a (n :: b) (Pro m :: c) d); intuition.
     + simpl. rewrite of_list_comm. unfold eq. simpl. fsetdec.
-  - simpl in *. simp mu in H0. specialize (H a b (Pro n :: l) d). intuition.
-    apply weaken. assumption.
-  - simpl in *. simp mu in H0. specialize (H a b (p :: Pro n :: l) (q :: d)). intuition.
-    apply Imp_R. assumption.
+  - simpl in *. simp mu in Hmu. apply weaken. specialize (H a b (Pro n :: l) d); intuition.
+  - simpl in *. simp mu in Hmu. apply Imp_R. specialize (H a b (p :: Pro n :: l) (q :: d)); intuition.
   - apply Fls_L.
   - apply Fls_L.
   - apply Fls_L.
   - apply Fls_L.
-  - simpl in *. simp mu in H1. assert (mu a b c [p] = [] /\ mu a b (q :: c) [] = []). { apply app_eq_nil. assumption. }
-    destruct H2. specialize (H a b c [p]). specialize (H0 a b (q :: c) []). intuition. apply Imp_L; assumption.
-  - simpl in *. simp mu in H0. specialize (H a (n :: b) (Imp p q :: l) d). intuition.
-    apply (Set_R (of_list (d ++ map Pro (n :: b)))).
-    + assumption.
+  - simpl in *. simp mu in Hmu.
+    assert (mu a b c [p] = [] /\ mu a b (q :: c) [] = []). { apply app_eq_nil. assumption. }
+    destruct Hmu. apply Imp_L. 
+    + apply (H a b c [p]); intuition.
+    + apply (H0 a b (q :: c) []); intuition.
+  - simpl in *. simp mu in Hmu. apply (Set_R (of_list (d ++ map Pro (n :: b)))).
+    + apply (H a (n :: b) (Imp p q :: l) d); intuition.
     + simpl. rewrite of_list_comm. simpl. unfold eq. fsetdec.
-  - simpl in *. simp mu in H0. specialize (H a b (Imp p q :: l) d). intuition.
-    apply weaken. assumption.
-  - simpl in *. simp mu in H0. specialize (H a b (p :: Imp r s :: c) (q :: d)). intuition.
-    apply Imp_R. assumption.
+  - simpl in *. simp mu in Hmu. apply weaken. apply (H a b (Imp p q :: l) d); intuition.
+  - simpl in *. simp mu in Hmu. apply Imp_R. apply (H a b (p :: Imp r s :: c) (q :: d)); intuition.
 Qed.
 
-Lemma mu_sound : forall a b c d, mu a b c d = [] -> forall i, sc (of_list (c ++ map Pro a)) (of_list (d ++ map Pro b)) i.
+Lemma mu_sound : forall a b c d,
+    mu a b c d = [] -> forall i, sc (of_list (c ++ map Pro a)) (of_list (d ++ map Pro b)) i.
 Proof.
   intros. apply sound_sc. apply proven. assumption.
 Qed.
 
-(* Equivalence between mu and mp *)
-
+(* To transfer these results to our boolean prover, we need an equivalence between mu and mp *)
 Lemma mu_mp_eq : forall a b c d, mu a b c d = [] <-> mp a b c d = true.
 Proof.
   split.
-  - intros. funelim (mu a b c d); simp mp; simp mu in *.
+  - intros H. funelim (mu a b c d); simp mp; simp mu in *.
     + destruct (common a b).
       * reflexivity.
       * inversion H.
@@ -437,18 +439,19 @@ Proof.
     + specialize (H a (n :: b) (Pro m :: c) d). intuition.
     + specialize (H a b (Pro n :: l) d). intuition.
     + specialize (H a b (p :: Pro n :: l) (q :: d)). intuition.
-    + reflexivity.
+    + intuition.
     + specialize (H a (n :: b) (Falsity :: l) d). intuition.
     + specialize (H a b (Falsity :: l) d). intuition.
     + specialize (H a b (p :: Falsity :: l) (q :: d)). intuition.
-    + assert (mu a b c [p] = [] /\ mu a b (q :: c) [] = []). { apply app_eq_nil. assumption. }
-      destruct H2. specialize (H a b c [p]). specialize (H0 a b (q :: c) []). intuition.
+    + assert (Hempty: mu a b c [p] = [] /\ mu a b (q :: c) [] = []).
+      { apply app_eq_nil. assumption. }
+      destruct Hempty. specialize (H a b c [p]). specialize (H0 a b (q :: c) []). intuition.
       rewrite H. assumption.        
     + specialize (H a (n :: b) (Imp p q :: l) d). intuition.
     + specialize (H a b (Imp p q :: l) d). intuition.
     + specialize (H a b (p :: Imp r s :: c) (q :: d)). intuition.
-  - intros. funelim (mp a b c d); simp mu; simp mp in *.
-    + rewrite H. reflexivity.
+  - intros H. funelim (mp a b c d); simp mu; simp mp in *.
+    + rewrite H. intuition.
     + specialize (H a (n :: b) [] d). intuition.
     + specialize (H a b [] d). intuition.
     + specialize (H a b [p] (q :: d)). intuition.
@@ -456,14 +459,14 @@ Proof.
     + specialize (H a (n :: b) (Pro m :: c) d). intuition.
     + specialize (H a b (Pro n :: l) d). intuition.
     + specialize (H a b (p :: Pro n :: l) (q :: d)). intuition.
-    + reflexivity.
+    + intuition.
     + specialize (H a (n :: b) (Falsity :: l) d). intuition.
     + specialize (H a b (Falsity :: l) d). intuition.
     + specialize (H a b (p :: Falsity :: l) (q :: d)). intuition.
-    + assert (mp a b (q :: c) [] = true /\ mp a b c [p] = true).
-      { destruct (mp a b (q :: c) []); destruct (mp a b c [p]); intuition. } destruct H2.
-      specialize (H a b c [p]). specialize (H0 a b (q :: c) []). intuition. rewrite H. rewrite H0.
-      reflexivity.
+    + assert (Htrue: mp a b (q :: c) [] = true /\ mp a b c [p] = true).
+      { destruct (mp a b (q :: c) []); destruct (mp a b c [p]); intuition. }
+      destruct Htrue. specialize (H a b c [p]). specialize (H0 a b (q :: c) []).
+      intuition. rewrite H. rewrite H0. reflexivity.
     + specialize (H a (n :: b) (Imp p q :: l) d). intuition.
     + specialize (H a b (Imp p q :: l) d). intuition.
     + specialize (H a b (p :: Imp r s :: c) (q :: d)). intuition.
@@ -471,60 +474,65 @@ Qed.
 
 (* Completeness *)
 
+(* We define an interpretation that checks for membership in a given set *)
 Definition counter_sem (ns : list nat) : (nat -> bool) :=
   fun n => member n ns.
 
-Lemma member_app : forall extra x xs, member x xs = true -> member x (extra ++ xs) = true.
+(* To prove completeness, we need a number of intermediate lemmas *)
+Lemma member_app : forall x xs extra, member x xs = true -> member x (extra ++ xs) = true.
 Proof.
-  intros. generalize dependent extra. induction xs.
-  - inversion H.
-  - intros. destruct (x =? a) eqn:Hax.
-    + apply member_In. apply Nat.eqb_eq in Hax. subst. intuition.
-    + simpl in H. rewrite Hax in H.
-      replace (extra ++ a :: xs) with ((extra ++ [a]) ++ xs) by (rewrite <- app_assoc; intuition).
-      apply (IHxs H (extra ++ [a])).
+  intros x xs. induction xs as [| x' xs' IH].
+  - intros extra H. inversion H.
+  - intros. destruct (x =? x') eqn:Heq.
+    + apply member_In. apply Nat.eqb_eq in Heq. subst. intuition.
+    + simpl in H. rewrite Heq in H.
+      replace (extra ++ x' :: xs') with ((extra ++ [x']) ++ xs') by (rewrite <- app_assoc; intuition).
+      apply (IH (extra ++ [x']) H).
 Qed.
 
-Lemma counter_lhs : forall extra a, For_all (semantics (counter_sem (extra ++ a))) (of_list (map Pro a)).
+Lemma counter_lhs : forall a extra, For_all (semantics (counter_sem (extra ++ a))) (of_list (map Pro a)).
 Proof.
-  unfold For_all. intros. generalize dependent extra. induction a.
-  - inversion H.
-  - intros. simpl in *. apply add_spec in H. destruct H.
-    + subst. simpl in *. unfold counter_sem in *. apply member_app. simpl. rewrite Nat.eqb_refl. reflexivity.
-    + replace (extra ++ a :: a0) with ((extra ++ [a]) ++ a0).
-      * apply IHa. assumption.
+  unfold For_all. intros a. induction a as [| a' as' IH].
+  - intros extra x H. inversion H.
+  - intros extra x H. simpl in *. apply add_spec in H. destruct H.
+    + subst. simpl in *. unfold counter_sem in *. apply member_app.
+      simpl. rewrite Nat.eqb_refl. reflexivity.
+    + replace (extra ++ a' :: as') with ((extra ++ [a']) ++ as').
+      * apply IH. assumption.
       * rewrite <- app_assoc. reflexivity.
 Qed.
 
-Lemma drop_falsity : forall a b i, sc a (add Falsity b) i -> sc a b i.
+Lemma drop_falsity : forall a b i, sc a (Falsity [+] b) i -> sc a b i.
 Proof.
-  unfold sc. intros. unfold Exists in *. specialize (H H0).
-  destruct H as [x [Hin Hx]]. exists x. intuition.
+  unfold sc. intros a b i Hsc Ha. unfold Exists in *. specialize (Hsc Ha).
+  destruct Hsc as [x [Hin Hx]]. exists x. intuition.
   apply add_spec in Hin. destruct Hin.
   - subst. contradiction.
   - assumption.
 Qed.
 
-Lemma sc_of_list_comm_right : forall x y z w i, sc x (add z (of_list (y ++ w))) i -> sc x (of_list (y ++ z :: w)) i.
+Lemma sc_of_list_comm_right : forall x y z w i,
+    sc x (add z (of_list (y ++ w))) i -> sc x (of_list (y ++ z :: w)) i.
 Proof.
-  unfold sc. unfold Exists. intros. specialize (H H0).
-  destruct H as [a [Hin Ha]]. exists a. split.
+  unfold sc. unfold Exists. intros x y z w i Hsc Hx. specialize (Hsc Hx).
+  destruct Hsc as [a [Hin Ha]]. exists a. split.
   - apply of_list_comm. assumption.
   - assumption.
 Qed.
 
-Lemma sc_of_list_comm_left : forall x y z w i,  sc (add x (of_list (y ++ z))) w i -> sc (of_list (y ++ x :: z)) w i.
+Lemma sc_of_list_comm_left : forall x y z w i,
+    sc (add x (of_list (y ++ z))) w i -> sc (of_list (y ++ x :: z)) w i.
 Proof.
-  unfold sc. unfold For_all. intros. apply H.
-  intros. apply H0. apply of_list_comm. assumption.
+  unfold sc. unfold For_all. intros x y z w i Hsc Hall. apply Hsc.
+  intros. apply Hall. apply of_list_comm. assumption.
 Qed.
 
 Lemma complete_imp_r : forall p q x y i, sc x (add (Imp p q) y) i -> sc (add p x) (add q y) i.
 Proof.
-  unfold sc. unfold Exists. unfold For_all. intros. destruct (semantics_dec i q).
+  unfold sc. unfold Exists. unfold For_all. intros p q x y i Hsc Hall. destruct (semantics_dec i q).
   - exists q. intuition.
-  - assert (Hasm: forall x0, In x0 x -> semantics i x0). { intros. apply H0. apply add_spec. intuition. }
-    specialize (H Hasm). destruct H as [e [Hin He]].
+  - assert (Hasm: forall x0, In x0 x -> semantics i x0). { intros. apply Hall. apply add_spec. intuition. }
+    destruct (Hsc Hasm) as [e [Hin He]].
     exists e. apply add_spec in Hin. split.
     + destruct (semantics_dec i p).
       * destruct Hin.
@@ -539,140 +547,162 @@ Qed.
 Lemma complete_imp_l : forall p q x y i, sc (add (Imp p q) x) y i -> sc x (add p y) i /\ sc (add q x) y i.
 Proof.
   unfold sc. unfold Exists. unfold For_all. split.
-  - intros. destruct (semantics_dec i p).
+  - intros Hall. destruct (semantics_dec i p).
     + exists p. intuition.
-    + destruct (semantics_dec i (Imp p q)).
+    + destruct (semantics_dec i (Imp p q)) as [ | Hsem].
       * assert (Hasm: forall x0, In x0 (add (Imp p q) x) -> semantics i x0).
-        { intros. apply add_spec in H3. destruct H3.
+        { intros a Ha. apply add_spec in Ha. destruct Ha.
           - subst. assumption.
           - intuition. }
         specialize (H Hasm). destruct H as [a [Hin Ha]].
         exists a. intuition.
-      * simpl in H2. intuition.
-  - intros. destruct (semantics_dec i q).
-    + destruct (semantics_dec i (Imp p q)).
-      * assert (Hasm: forall x0, In x0 x -> semantics i x0). { intros. apply H0. intuition. }
-        apply H. intros. apply add_spec in H3. destruct H3.
+      * simpl in Hsem. intuition.
+  - intros Hall. destruct (semantics_dec i q).
+    + destruct (semantics_dec i (Imp p q)) as [ | Hsem].
+      * assert (Hasm: forall x0, In x0 x -> semantics i x0). { intros. apply Hall. intuition. }
+        apply H. intros a Ha. apply add_spec in Ha. destruct Ha.
         -- subst. assumption.
         -- intuition.
-      * simpl in H2. intuition.
+      * simpl in Hsem. intuition.
     + intuition.
 Qed.
 
 Lemma member_common : forall a x y, member a x = true -> member a y = true -> common x y = true.
 Proof.
-  intros a x. induction y.
+  intros a x y. induction y as [| a' as' IH ].
   - intros. inversion H0.
-  - intros. simpl. destruct (a =? a0) eqn:Heq.
-    + apply Nat.eqb_eq in Heq. subst. rewrite H. reflexivity.
-    + simpl in H0. rewrite Heq in H0. specialize (IHy H H0).
-      rewrite IHy. destruct (member a0 x); intuition.
+  - intros Hx Hy. simpl. destruct (a =? a') eqn:Heq.
+    + apply Nat.eqb_eq in Heq. subst. rewrite Hx. reflexivity.
+    + simpl in Hy. rewrite Heq in Hy. specialize (IH Hx Hy).
+      rewrite IH. destruct (member a' x); intuition.
 Qed.
 
 Lemma in_of_list_member : forall x xs, In (Pro x) (of_list (map Pro xs)) -> member x xs = true.
 Proof.
-  intros. induction xs.
+  intros x xs H. induction xs as [| x' xs' IH].
   - inversion H.
-  - simpl. destruct (x =? a) eqn:Heq.
+  - simpl. destruct (x =? x') eqn:Heq.
     + reflexivity.
-    + apply IHxs. simpl in H. apply add_spec in H. destruct H.
+    + apply IH. simpl in H. apply add_spec in H. destruct H.
       * apply Nat.eqb_neq in Heq. inversion H. contradiction.
       * assumption.
 Qed.
 
 Lemma in_map_inversion : forall x xs, In x (of_list (map Pro xs)) -> exists y, x = Pro y /\ List.In y xs.
 Proof.
-  intros. induction xs.
+  intros x xs H. induction xs as [| x' xs' IH].
   - inversion H.
   - simpl in H. apply add_spec in H. destruct H.
-    + exists a. intuition.
-    + specialize (IHxs H). destruct IHxs as [y [Hxy Hin]].
+    + exists x'. intuition.
+    + specialize (IH H). destruct IH as [y [Hxy Hin]].
       exists y. intuition.
 Qed.
-    
-Lemma counter : forall a b c d (xs : list nat), List.In xs (mu a b c d) -> ~ sc (of_list (c ++ map Pro a)) (of_list (d ++ map Pro b)) (counter_sem xs).
+
+(* Under the interpretation defined above, the prover returns counterexamples
+   if it returns a non-empty list *)
+Lemma counter : forall a b c d (xs : list nat),
+    List.In xs (mu a b c d) ->
+    ~ sc (of_list (c ++ map Pro a)) (of_list (d ++ map Pro b)) (counter_sem xs).
 Proof.
-  intros. funelim (mu a b c d).
-  - simpl in *. simp mu in H. destruct (common a b) eqn:Hab.
-    + inversion H.
-    + inversion H.
-      * subst. unfold sc. unfold not. intros. specialize (H0 (counter_lhs [] xs)).
-        unfold Exists in H0. destruct H0 as [x [Hin Hx]].
+  intros a b c d xs Hin. funelim (mu a b c d).
+  - simpl in *. simp mu in Hin. destruct (common a b) eqn:Hab.
+    + inversion Hin.
+    + inversion Hin as [H | H].
+      * subst. unfold sc. unfold not. intros. specialize (H (counter_lhs xs [])).
+        unfold Exists in H. destruct H as [x [Hin' Hx]].
         assert (exists x', x = Pro x').
-        { apply in_map_inversion in Hin. destruct Hin as [y [Hxy Hin]]. exists y. intuition. }
-        destruct H0 as [x' Hx']. subst. simpl in *.
-        apply in_of_list_member in Hin.
+        { apply in_map_inversion in Hin'. destruct Hin' as [y [Hxy Hin']]. exists y. intuition. }
+        destruct H as [x' Hx']. subst. simpl in *.
+        apply in_of_list_member in Hin'.
         assert (common xs b = true). apply (member_common x'); assumption.
         congruence.
       * contradiction.
-  - simpl in *. simp mu in H0. specialize (H xs H0). unfold not. intros. apply H.
-    apply sc_of_list_comm_right. assumption.
-  - simpl in *. simp mu in H0. specialize (H xs H0). unfold not. intros. apply drop_falsity in H1.
-    intuition.
-  - simpl in *. simp mu in H0. specialize (H xs H0). unfold not. intros. apply H.
-    apply complete_imp_r. assumption.
-  - simpl in *. simp mu in H0. specialize (H xs H0). unfold not. intros. apply H.
-    apply sc_of_list_comm_left. assumption.
-  - simpl in *. simp mu in H0. specialize (H xs H0). unfold not. intros. apply H.
-    apply sc_of_list_comm_right. assumption.
-  - simpl in *. simp mu in H0. specialize (H xs H0). unfold not. intros. apply drop_falsity in H1.
-    intuition.
-  - simpl in *. simp mu in H0. specialize (H xs H0). unfold not. intros. apply H.
-    apply complete_imp_r. assumption.
-  - simp mu in H. inversion H.
-  - simpl in *. simp mu in H0. specialize (H xs H0). unfold not. intros. apply H.
-    apply sc_of_list_comm_right. assumption.
-  - simpl in *. simp mu in H0. specialize (H xs H0). unfold not. intros. apply drop_falsity in H1.
-    intuition.
-  - simpl in *. simp mu in H0. specialize (H xs H0). unfold not. intros. apply H.
-    apply complete_imp_r. assumption.
-  - simpl in *. simp mu in H1. apply in_app_or in H1. destruct H1.
-    + specialize (H xs H1). unfold not. intros. apply H. apply complete_imp_l in H2. intuition.
-    + specialize (H0 xs H1). unfold not. intros. apply H0. apply complete_imp_l in H2. intuition.
-  - simpl in *. simp mu in H0. specialize (H xs H0). unfold not. intros. apply H.
-    apply sc_of_list_comm_right. assumption.
-  - simpl in *. simp mu in H0. specialize (H xs H0). unfold not. intros. apply drop_falsity in H1.
-    intuition.
-  - simpl in *. simp mu in H0. specialize (H xs H0). unfold not. intros. apply H.
-    apply complete_imp_r. assumption.
+  - simpl in *. simp mu in Hin. specialize (H xs Hin). unfold not. intros.
+    apply H. apply sc_of_list_comm_right. assumption.
+  - simpl in *. simp mu in Hin. specialize (H xs Hin). unfold not. intros Hsc.
+    apply drop_falsity in Hsc. intuition.
+  - simpl in *. simp mu in Hin. specialize (H xs Hin). unfold not. intros.
+    apply H. apply complete_imp_r. assumption.
+  - simpl in *. simp mu in Hin. specialize (H xs Hin). unfold not. intros.
+    apply H. apply sc_of_list_comm_left. assumption.
+  - simpl in *. simp mu in Hin. specialize (H xs Hin). unfold not. intros.
+    apply H. apply sc_of_list_comm_right. assumption.
+  - simpl in *. simp mu in Hin. specialize (H xs Hin). unfold not. intros Hsc.
+    apply drop_falsity in Hsc. intuition.
+  - simpl in *. simp mu in Hin. specialize (H xs Hin). unfold not. intros.
+    apply H. apply complete_imp_r. assumption.
+  - simp mu in Hin. inversion Hin.
+  - simpl in *. simp mu in Hin. specialize (H xs Hin). unfold not. intros.
+    apply H. apply sc_of_list_comm_right. assumption.
+  - simpl in *. simp mu in Hin. specialize (H xs Hin). unfold not. intros Hsc.
+    apply drop_falsity in Hsc. intuition.
+  - simpl in *. simp mu in Hin. specialize (H xs Hin). unfold not. intros.
+    apply H. apply complete_imp_r. assumption.
+  - simpl in *. simp mu in Hin. apply in_app_or in Hin. destruct Hin as [Hin | Hin].
+    + specialize (H xs Hin). unfold not. intros Hsc. apply H. apply complete_imp_l in Hsc. intuition.
+    + specialize (H0 xs Hin). unfold not. intros Hsc. apply H0. apply complete_imp_l in Hsc. intuition.
+  - simpl in *. simp mu in Hin. specialize (H xs Hin). unfold not. intros.
+    apply H. apply sc_of_list_comm_right. assumption.
+  - simpl in *. simp mu in Hin. specialize (H xs Hin). unfold not. intros Hsc.
+    apply drop_falsity in Hsc. intuition.
+  - simpl in *. simp mu in Hin. specialize (H xs Hin). unfold not. intros.
+    apply H. apply complete_imp_r. assumption.
 Qed.
 
-Lemma mu_complete : forall a b c d, (forall i, sc (of_list (c ++ map Pro a)) (of_list (d ++ map Pro b)) i) -> mu a b c d = [].
+(* Thus the prover must return an empty list for any valid formula *)
+Lemma mu_complete : forall a b c d,
+    (forall i, sc (of_list (c ++ map Pro a)) (of_list (d ++ map Pro b)) i) -> mu a b c d = [].
 Proof.
-  intros. destruct (mu a b c d) eqn:He.
+  intros a b c d H. destruct (mu a b c d) eqn:He.
   - reflexivity.
   - exfalso. specialize counter. intros counter.
-    specialize (counter a b c d l). unfold not in counter.
-    apply counter.
+    specialize (counter a b c d l). unfold not in counter. apply counter.
     + rewrite He. apply in_eq.
     + apply H.
 Qed.
 
-Theorem sound_complete' : forall a b c d, (forall i, sc (of_list (c ++ map Pro a)) (of_list (d ++ map Pro b)) i) <-> mp a b c d = true.
+(* Using the equivalence and the results until now, we reach our main theorem:
+   The boolean prover returns true exactly when the sequent is provable. *)
+Theorem sound_complete' : forall a b c d,
+    (forall i, sc (of_list (c ++ map Pro a)) (of_list (d ++ map Pro b)) i) <-> mp a b c d = true.
 Proof.
   unfold prover. split.
   - intros. apply mu_mp_eq. apply mu_complete. assumption.
-  - intros. apply mu_mp_eq in H. apply mu_sound. assumption.
+  - intros H. apply mu_mp_eq in H. apply mu_sound. assumption.
 Qed.
 
-Lemma sc_semantics : forall i p, sc (of_list ([] ++ map Pro [])) (of_list ([p] ++ map Pro [])) i -> semantics i p.
+(* We can also specialize this to single formulas: *)
+Lemma sc_semantics : forall i p,
+    sc (of_list ([] ++ map Pro [])) (of_list ([p] ++ map Pro [])) i -> semantics i p.
 Proof.
-  intros. simpl in H. unfold sc in H. unfold Exists in H. unfold For_all in H.
-  assert (forall x, In x empty -> semantics i x). { intros. inversion H0. }
-  specialize (H H0). destruct H as [x [Hadd Hx]]. apply add_spec in Hadd. destruct Hadd.
+  intros i p H. simpl in H. unfold sc in H. unfold Exists in H. unfold For_all in H.
+  assert (Hempty: forall x, In x empty -> semantics i x). { intros. inversion H0. }
+  specialize (H Hempty). destruct H as [x [Hadd Hx]]. apply add_spec in Hadd. destruct Hadd.
   - subst. assumption.
   - inversion H.
 Qed.
 
+(* We thus reach our main result for the final prover:
+   The prover for single formulas returns true exactly when the given formula is valid. *)
 Corollary sound_complete : forall p, (forall i, semantics i p) <-> prover p = true.
 Proof.
   intros p. split.
   - intros H. apply sound_complete'. intros i. unfold sc. simpl.
-    intros Hs. unfold For_all in Hs. unfold Exists. exists p; intuition.
-  - intros. unfold prover in H. apply sc_semantics. apply sound_complete'. assumption.
+    intros Hall. unfold For_all in Hall. unfold Exists. exists p; intuition.
+  - intros H i. unfold prover in H. apply sc_semantics. apply sound_complete'. assumption.
 Qed.
 
+(* We can now extract our final prover to Haskell to integrate it into an application *)
 Extraction Language Haskell.
+
+(* To fit into Haskell easily, we translate the Coq definitions of standard concepts
+   into the native Haskell equivalents.
+   Concretely, we translate list into Haskell lists, bool into Haskell booleans and
+   nat into the Int type in Haskell.
+   All of this can be set up by importing the following standard translation packages:
+ *)
 Require Import ExtrHaskellBasic.
 Require Import ExtrHaskellNatInt.
+
+(* We then extract the prover function into a Haskell library module: *)
 Extraction "prover/MicroProver.hs" prover.
